common/Memory.v
@@ -101,5 +101,7 @@ Hint Resolve
   Mem.valid_access_free_inv_1
   Mem.valid_access_free_inv_2
   Mem.unchanged_on_refl
+  Mem.push_frame_valid_block_1
+  Mem.push_frame_perm_1
 : mem.
 
